finish spec equiv proof of hacl.spec.sha2.hash == spec.agile.hash.hash

code/sha2-vec/Hacl.Spec.SHA2.EquivScalar.fst
@@ -21,10 +21,311 @@ friend Spec.Agile.Hash
 
 #set-options "--z3rlimit 50 --fuel 0 --ifuel 0"
 
+val ws_next_inductive: a:sha2_alg -> ws0:k_w a -> k:nat{k <= 16} ->
+  Pure (k_w a)
+  (requires True)
+  (ensures fun res ->
+    res == Loops.repeati k (ws_next_inner a) ws0 /\
+    (forall (i:nat{i < k}). index res i == index (ws_next_inner a i (Loops.repeati i (ws_next_inner a) ws0)) i) /\
+    (forall (i:nat{i < k - 1}). index res i == index (Loops.repeati (k - 1) (ws_next_inner a) ws0) i) /\
+    (forall (i:nat{k <= i /\ i < 16}). index res i == index ws0 i))
+
+let ws_next_inductive a ws0 k =
+  Loops.eq_repeati0 k (ws_next_inner a) ws0;
+  repeati_inductive #(k_w a) k
+  (fun i wsi ->
+    wsi == Loops.repeati i (ws_next_inner a) ws0 /\
+   (forall (i0:nat{i0 < i}). index wsi i0 == index (ws_next_inner a i0 (Loops.repeati i0 (ws_next_inner a) ws0)) i0) /\
+   (forall (i0:nat{i0 < i - 1}). index wsi i0 == index (Loops.repeati (i - 1) (ws_next_inner a) ws0) i0) /\
+   (forall (i0:nat{i <= i0 /\ i0 < 16}). index wsi i0 == index ws0 i0))
+  (fun i wsi ->
+    let ws = ws_next_inner a i wsi in
+    Loops.unfold_repeati (i + 1) (ws_next_inner a) ws0 i;
+    ws)
+  ws0
+
+
+val ws_next_lemma: a:sha2_alg -> ws0:k_w a -> k:pos{k <= 16} -> Lemma
+  (let wsk : k_w a = Loops.repeati k (ws_next_inner a) ws0 in
+   let wsk1 : k_w a = Loops.repeati (k - 1) (ws_next_inner a) ws0 in
+   (forall (i:nat{i < k}). index wsk i == index (ws_next_inner a i (Loops.repeati i (ws_next_inner a) ws0)) i) /\
+   (forall (i:nat{i < k - 1}). index wsk i == index wsk1 i) /\
+   (forall (i:nat{k <= i /\ i < 16}). index wsk i == index ws0 i))
+
+let ws_next_lemma a ws0 k =
+  let _ = ws_next_inductive a ws0 k in ()
+
+
+val ws_next_lemma_k: a:sha2_alg -> ws0:k_w a -> k:nat{k < 16} -> Lemma
+  (let ws : k_w a = Loops.repeati 16 (ws_next_inner a) ws0 in
+  let wsk : k_w a = Loops.repeati (k + 1) (ws_next_inner a) ws0 in
+  Seq.index ws k == Seq.index wsk k)
+
+let ws_next_lemma_k a ws0 k =
+  ws_next_lemma a ws0 (k + 1);
+  ws_next_lemma a ws0 16
+
+
+val ws_pre_inductive: a:sha2_alg -> block:Spec.block_w a -> k:nat{k <= Spec.size_k_w a} ->
+  Pure (Spec.k_w a)
+  (requires True)
+  (ensures  fun res ->
+   (let ws0 = Seq.create (Spec.size_k_w a) (to_word a 0) in
+    res == Loops.repeati k (Spec.ws_pre_inner a block) ws0 /\
+    (forall (i:nat{i < k}).
+      Seq.index res i ==
+      Seq.index (Spec.ws_pre_inner a block i (Loops.repeati (i + 1) (Spec.ws_pre_inner a block) ws0)) i) /\
+    (forall (i:nat{i < k - 1}).
+      Seq.index res i == Seq.index (Loops.repeati (k - 1) (Spec.ws_pre_inner a block) ws0) i) /\
+    (forall (i:nat{k <= i /\ i < Spec.size_k_w a}). Seq.index res i == Seq.index ws0 i)))
+
+let ws_pre_inductive a block k =
+  let ws0 = Seq.create (Spec.size_k_w a) (to_word a 0) in
+  Loops.eq_repeati0 k (Spec.ws_pre_inner a block) ws0;
+  repeati_inductive #(Spec.k_w a) k
+  (fun i wsi ->
+    wsi == Loops.repeati i (Spec.ws_pre_inner a block) ws0 /\
+   (forall (i0:nat{i0 < i}).
+     Seq.index wsi i0 ==
+     Seq.index (Spec.ws_pre_inner a block i0 (Loops.repeati (i0 + 1) (Spec.ws_pre_inner a block) ws0)) i0) /\
+   (forall (i0:nat{i0 < i - 1}). Seq.index wsi i0 == Seq.index (Loops.repeati (i - 1) (Spec.ws_pre_inner a block) ws0) i0) /\
+   (forall (i0:nat{i <= i0 /\ i0 < Spec.size_k_w a}). Seq.index wsi i0 == Seq.index ws0 i0))
+  (fun i wsi ->
+    let ws = Spec.ws_pre_inner a block i wsi in
+    Loops.unfold_repeati (i + 1) (Spec.ws_pre_inner a block) ws0 i;
+    ws)
+  ws0
+
+
+val ws_pre_lemma: a:sha2_alg -> block:Spec.block_w a -> k:pos{k <= Spec.size_k_w a} -> Lemma
+  (let ws0 = Seq.create (Spec.size_k_w a) (to_word a 0) in
+   let wsk : Spec.k_w a = Loops.repeati k (Spec.ws_pre_inner a block) ws0 in
+   let wsk1 : Spec.k_w a = Loops.repeati (k - 1) (Spec.ws_pre_inner a block) ws0 in
+  (forall (i:nat{i < k}).
+    Seq.index wsk i ==
+    Seq.index (Spec.ws_pre_inner a block i (Loops.repeati (i + 1) (Spec.ws_pre_inner a block) ws0)) i) /\
+  (forall (i:nat{i < k - 1}). Seq.index wsk i == Seq.index wsk1 i) /\
+  (forall (i:nat{k <= i /\ i < Spec.size_k_w a}). Seq.index wsk i == Seq.index ws0 i))
+
+let ws_pre_lemma a block k =
+  let _ = ws_pre_inductive a block k in ()
+
+
+val ws_pre_lemma_k: a:sha2_alg -> block:Spec.block_w a -> k:nat{k < Spec.size_k_w a} -> Lemma
+  (let ws0 = Seq.create (Spec.size_k_w a) (to_word a 0) in
+   let ws : Spec.k_w a = Loops.repeati (Spec.size_k_w a) (Spec.ws_pre_inner a block) ws0 in
+   let wsk : Spec.k_w a = Loops.repeati (k + 1) (Spec.ws_pre_inner a block) ws0 in
+   Seq.index wsk k == Seq.index ws k)
+
+let ws_pre_lemma_k a block k =
+  ws_pre_lemma a block (k + 1);
+  ws_pre_lemma a block (Spec.size_k_w a)
+
+
+val ws_next_pre_lemma_j_step:
+    a:sha2_alg
+  -> block:Spec.block_w a
+  -> i:nat{i < num_rounds16 a - 1}
+  -> j:nat{j < 16}
+  -> ws1:Spec.k_w a
+  -> ws_n1:k_w a ->
+  Lemma
+  (requires
+   (let ws_n0 : k_w a = Seq.slice ws1 (16 * i) (16 * i + 16) in
+    Seq.slice ws_n1 0 j == Seq.slice ws1 (16 * i + 16) (16 * i + 16 + j) /\
+    Seq.slice ws_n1 j 16 == Seq.slice ws_n0 j 16))
+  (ensures
+    (let ws_n = ws_next_inner a j ws_n1 in
+     let ws = Spec.ws_pre_inner a block (16 * i + 16 + j) ws1 in
+     Seq.index ws_n j == Seq.index ws (16 * i + 16 + j)))
+
+let ws_next_pre_lemma_j_step a block i j ws1 ws_n1 =
+  let ws_n = ws_next_inner a j ws_n1 in
+  let ws = Spec.ws_pre_inner a block (16 * i + 16 + j) ws1 in
+
+  let s0_n = _sigma0 a ws_n1.[(j+1) % 16] in
+  let s1_n = _sigma1 a ws_n1.[(j+14) % 16] in
+  //assert (Seq.index ws_n j == s1_n +. ws_n1.[(j+9) % 16] +. s0_n +. ws_n1.[j]);
+
+  let s0 = _sigma0 a ws1.[16 * i + 16 + j - 15] in
+  let s1 = _sigma1 a ws1.[16 * i + 16 + j - 2] in
+  //assert (Seq.index ws (16 * i + 16 + j) == s1 +. ws1.[16 * i + 16 + j - 7] +. s0 +. ws1.[16 * i + 16 + j - 16]);
+
+  let ws_n1_index (k:nat{k < 16}) :
+    Lemma (if k < j then ws_n1.[k] == ws1.[16 * i + 16 + k] else ws_n1.[k] == ws1.[16 * i + k]) =
+    if k < j then Seq.lemma_index_slice ws_n1 0 j k
+    else Seq.lemma_index_slice ws_n1 j 16 (k - j) in
+
+  ws_n1_index ((j + 1) % 16);
+  assert (ws_n1.[(j + 1) % 16] == ws1.[16 * i + j + 1]);
+  ws_n1_index ((j + 14) % 16);
+  assert (ws_n1.[(j + 14) % 16] == ws1.[16 * i + j + 14]);
+  ws_n1_index ((j + 9) % 16);
+  assert (ws_n1.[(j + 9) % 16] == ws1.[16 * i + j + 9]);
+  ws_n1_index j;
+  assert (ws_n1.[j] == ws1.[16 * i + j])
+
+
+val ws_next_pre_lemma_aux:
+    a:sha2_alg
+  -> i:nat{i < num_rounds16 a - 1}
+  -> j:pos{j <= 16}
+  -> ws1:Spec.k_w a
+  -> ws_n1:k_w a
+  -> ws:Spec.k_w a
+  -> ws_n:k_w a ->
+  Lemma
+  (requires
+   (let ws_n0 : k_w a = Seq.slice ws (16 * i) (16 * i + 16) in
+    Seq.slice ws_n1 0 (j - 1) == Seq.slice ws1 (16 * i + 16) (16 * i + 16 + j - 1) /\
+    (forall (k:nat{k < 16 * i + 16 + j - 1}). Seq.index ws k == Seq.index ws1 k) /\
+    (forall (k:nat{k < j - 1}). Seq.index ws_n k == Seq.index ws_n1 k) /\
+    Seq.index ws_n (j - 1) == Seq.index ws (16 * i + 16 + j - 1) /\
+    (forall (k:nat{j <= k /\ k < 16}). Seq.index ws_n k == Seq.index ws_n0 k)))
+  (ensures
+   (let ws_n0 : k_w a = Seq.slice ws (16 * i) (16 * i + 16) in
+    Seq.slice ws_n 0 j == Seq.slice ws (16 * i + 16) (16 * i + 16 + j) /\
+    Seq.slice ws_n j 16 == Seq.slice ws_n0 j 16))
+
+let ws_next_pre_lemma_aux a i j ws1 ws_n1 ws ws_n =
+  let ws_n0 : k_w a = Seq.slice ws (16 * i) (16 * i + 16) in
+  assert (Seq.slice ws_n1 0 (j - 1) == Seq.slice ws1 (16 * i + 16) (16 * i + 16 + j - 1));
+
+  let ws_n1_index1 (k:nat{k < j - 1}) : Lemma (Seq.index ws_n1 k == Seq.index ws1 (16 * i + 16 + k)) =
+    Seq.lemma_index_slice ws_n1 0 (j - 1) k;
+    Seq.lemma_index_slice ws1 (16 * i + 16) (16 * i + 16 + j - 1) k in
+
+  let ws_n_index1 (k:nat{k < j}) : Lemma (Seq.index ws_n k == Seq.index ws (16 * i + 16 + k)) =
+    if k < j - 1 then ws_n1_index1 k else () in
+
+  let ws_n_index2 (k:nat{j <= k /\ k < 16}) : Lemma (Seq.index ws_n k == Seq.index ws_n0 k) =
+    () in
+
+  Classical.forall_intro ws_n_index1;
+  Seq.lemma_eq_intro (Seq.slice ws_n 0 j) (Seq.slice ws (16 * i + 16) (16 * i + 16 + j));
+  Classical.forall_intro ws_n_index2;
+  Seq.lemma_eq_intro (Seq.slice ws_n j 16) (Seq.slice ws_n0 j 16)
+
+
+val ws_next_pre_lemma_init:
+    a:sha2_alg
+  -> block:Spec.block_w a
+  -> i:nat{i < num_rounds16 a - 1}
+  -> j:pos{j <= 16} -> Lemma
+  (let ws0 = Seq.create (Spec.size_k_w a) (to_word a 0) in
+   let ws : Spec.k_w a = Loops.repeati (16 * i + 16 + j) (Spec.ws_pre_inner a block) ws0 in
+   let ws1 : Spec.k_w a = Loops.repeati (16 * i + 16 + j - 1) (Spec.ws_pre_inner a block) ws0 in
+   Seq.slice ws1 (16 * i) (16 * i + 16) == Seq.slice ws (16 * i) (16 * i + 16))
+
+let ws_next_pre_lemma_init a block i j =
+  let ws0 = Seq.create (Spec.size_k_w a) (to_word a 0) in
+  let ws : Spec.k_w a = Loops.repeati (16 * i + 16 + j) (Spec.ws_pre_inner a block) ws0 in
+  let ws1 : Spec.k_w a = Loops.repeati (16 * i + 16 + j - 1) (Spec.ws_pre_inner a block) ws0 in
+
+  let s : Spec.block_w a = Seq.slice ws (16 * i) (16 * i + 16) in
+  let s1 : Spec.block_w a = Seq.slice ws1 (16 * i) (16 * i + 16) in
+
+  let aux (k:nat{k < 16}) : Lemma (Seq.index s k == Seq.index s1 k) =
+    ws_pre_lemma a block (16 * i + 16 + j);
+    ws_pre_lemma a block (16 * i + 16 + j - 1) in
+
+  Classical.forall_intro aux;
+  Seq.lemma_eq_intro s s1
+
+
+val ws_next_pre_lemma_j:
+    a:sha2_alg
+  -> block:Spec.block_w a
+  -> i:nat{i < num_rounds16 a - 1}
+  -> j:nat{j <= 16} -> Lemma
+  (let ws0 = Seq.create (Spec.size_k_w a) (to_word a 0) in
+   let ws : Spec.k_w a = Loops.repeati (16 * i + 16 + j) (Spec.ws_pre_inner a block) ws0 in
+   let ws_n0 : k_w a = Seq.slice ws (16 * i) (16 * i + 16) in
+   let ws_n : k_w a = Loops.repeati j (ws_next_inner a) ws_n0 in
+   Seq.slice ws_n 0 j == Seq.slice ws (16 * i + 16) (16 * i + 16 + j) /\
+   Seq.slice ws_n j 16 == Seq.slice ws_n0 j 16)
+
+let rec ws_next_pre_lemma_j a block i j =
+  let ws_pre_f = Spec.ws_pre_inner a block in
+  let ws_next_f = ws_next_inner a in
+
+  let ws0 = Seq.create (Spec.size_k_w a) (to_word a 0) in
+  let ws : Spec.k_w a = Loops.repeati (16 * i + 16 + j) ws_pre_f ws0 in
+  let ws_n0 : k_w a = Seq.slice ws (16 * i) (16 * i + 16) in
+  let ws_n : k_w a = Loops.repeati j ws_next_f ws_n0 in
+
+  if j = 0 then
+    Loops.eq_repeati0 j ws_next_f ws_n0
+  else begin
+    let ws1 : Spec.k_w a = Loops.repeati (16 * i + 16 + j - 1) ws_pre_f ws0 in
+    ws_next_pre_lemma_init a block i j;
+    assert (Seq.slice ws1 (16 * i) (16 * i + 16) == ws_n0);
+    let ws_n1 : k_w a  = Loops.repeati (j - 1) ws_next_f ws_n0 in
+    ws_next_pre_lemma_j a block i (j - 1);
+    assert (Seq.slice ws_n1 0 (j - 1) == Seq.slice ws1 (16 * i + 16) (16 * i + 16 + j - 1));
+    assert (Seq.slice ws_n1 (j - 1) 16 == Seq.slice ws_n0 (j - 1) 16);
+
+    ws_pre_lemma a block (16 * i + 16 + j);
+    assert (forall (k:nat{k < 16 * i + 16 + j - 1}). Seq.index ws k == Seq.index ws1 k);
+    Loops.unfold_repeati (16 * i + 16 + j) ws_pre_f ws0 (16 * i + 16 + j - 1);
+    //assert (ws == ws_pre_f (16 * i + 16 + j - 1) ws1);
+
+    ws_next_lemma a ws_n0 j;
+    assert (forall (k:nat{k < j - 1}). Seq.index ws_n k == Seq.index ws_n1 k);
+    assert (forall (k:nat{j <= k /\ k < 16}). Seq.index ws_n k == Seq.index ws_n0 k);
+    Loops.unfold_repeati j ws_next_f ws_n0 (j - 1);
+    //assert (ws_n == ws_next_f (j - 1) ws_n1);
+    ws_next_pre_lemma_j_step a block i (j - 1) ws1 ws_n1;
+    assert (Seq.index ws_n (j - 1) == Seq.index ws (16 * i + 16 + j - 1));
+    ws_next_pre_lemma_aux a i j ws1 ws_n1 ws ws_n;
+    () end
+
+
+val ws_next_pre_lemma:
+    a:sha2_alg
+  -> block:Spec.block_w a
+  -> i:nat{i < num_rounds16 a - 1}
+  -> j:nat{j < 16} -> Lemma
+  (let ws : Spec.k_w a = Spec.ws_pre a block in
+   let ws_n0 : k_w a = Seq.slice ws (16 * i) (16 * i + 16) in
+   let ws_n : k_w a = ws_next a ws_n0 in
+   Seq.index ws_n j == Seq.index ws (16 * i + 16 + j))
+
+let ws_next_pre_lemma a block i j =
+  reveal_opaque (`%Spec.ws_pre) Spec.ws_pre;
+  let ws0 = Seq.create (Spec.size_k_w a) (to_word a 0) in
+  let ws : Spec.k_w a = Loops.repeati (Spec.size_k_w a) (Spec.ws_pre_inner a block) ws0 in
+  let ws_n0 : k_w a = Seq.slice ws (16 * i) (16 * i + 16) in
+  let ws_n : k_w a = Loops.repeati 16 (ws_next_inner a) ws_n0 in
+
+  let wsj : Spec.k_w a = Loops.repeati (16 * i + 16 + j + 1) (Spec.ws_pre_inner a block) ws0 in
+  let ws_n0j : k_w a = Seq.slice wsj (16 * i) (16 * i + 16) in
+  let ws_nj : k_w a = Loops.repeati (j + 1) (ws_next_inner a) ws_n0 in
+
+  let aux (k:nat{k < 16}) : Lemma (Seq.index ws_n0 k == Seq.index ws_n0j k) =
+    ws_pre_lemma a block (16 * i + 16 + j + 1);
+    ws_pre_lemma a block (Spec.size_k_w a) in
+
+  Classical.forall_intro aux;
+  Seq.lemma_eq_intro ws_n0 ws_n0j;
+
+  ws_next_pre_lemma_j a block i (j + 1);
+  assert (Seq.slice ws_nj 0 (j + 1) == Seq.slice wsj (16 * i + 16) (16 * i + 16 + j + 1));
+  Seq.lemma_index_slice ws_nj 0 (j + 1) j;
+  assert (Seq.index ws_nj j == Seq.index wsj (16 * i + 16 + j));
+
+  ws_pre_lemma_k a block (16 * i + 16 + j);
+  assert (Seq.index wsj (16 * i + 16 + j) == Seq.index ws (16 * i + 16 + j));
+
+  ws_next_lemma_k a ws_n0 j;
+  assert (Seq.index ws_nj j == Seq.index ws_n j)
+
+
 val shuffle_core_pre_lemma: a:sha2_alg -> k_t:word a -> ws_t:word a -> hash:words_state a ->
   Lemma (shuffle_core_pre a k_t ws_t hash == Spec.shuffle_core_pre a k_t ws_t hash)
 let shuffle_core_pre_lemma a k_t ws_t hash =
   reveal_opaque (`%Spec.shuffle_core_pre) Spec.shuffle_core_pre
+
 
 noextract
 val shuffle_pre_inner: a:sha2_alg -> ws:Spec.k_w a -> i:nat{i < size_k_w a} -> st:words_state a -> words_state a
@@ -128,34 +429,93 @@ let shuffle_spec_lemma16 a st0 block =
     st0
 
 
+val ws_next_inner_lemma:
+    a:sha2_alg
+  -> block:k_w a
+  -> i:nat{i < num_rounds16 a}
+  -> ws1:k_w a ->
+  Lemma
+  (requires
+   (let ws_s = Spec.ws_pre a block in
+   (if i < num_rounds16 a - 1 then
+      ws1 == Seq.slice ws_s (16 * i) (16 * i + 16)
+    else
+      ws1 == Seq.slice ws_s (16 * (num_rounds16 a - 1)) (16 * num_rounds16 a))))
+  (ensures
+   (let ws_s = Spec.ws_pre a block in
+    let ws = if i < num_rounds16 a - 1 then ws_next a ws1 else ws1 in
+   (if i < num_rounds16 a - 1 then
+      ws == Seq.slice ws_s (16 * (i + 1)) (16 * (i + 1) + 16)
+    else
+      ws == Seq.slice ws_s (16 * (num_rounds16 a - 1)) (16 * num_rounds16 a))))
+
+let ws_next_inner_lemma a block i ws1 =
+  let ws_s : Spec.k_w a = Spec.ws_pre a block in
+  let ws = if i < num_rounds16 a - 1 then ws_next a ws1 else ws1 in
+
+  if i < num_rounds16 a - 1 then begin
+    let aux (k:nat{k < 16}) : Lemma (Seq.index (ws_next a ws1) k == Seq.index ws_s (16 * (i + 1) + k)) =
+      ws_next_pre_lemma a block i k in
+    Classical.forall_intro aux;
+    Seq.lemma_eq_intro (ws_next a ws1) (Seq.slice ws_s (16 * (i + 1)) (16 * (i + 1) + 16)) end
+  else ()
+
+
 val shuffle_lemma_i_step:
     a:sha2_alg
   -> block:k_w a
   -> st0:words_state a
   -> i:nat{i < num_rounds16 a}
   -> ws1:k_w a
-  -> st1:words_state a -> Lemma
+  -> st1:words_state a ->
+  Lemma
+  (requires
+   (let ws_s = Spec.ws_pre a block in
+   (if i < num_rounds16 a - 1 then
+      ws1 == Seq.slice ws_s (16 * i) (16 * i + 16)
+    else
+      ws1 == Seq.slice ws_s (16 * (num_rounds16 a - 1)) (16 * num_rounds16 a))))
+  (ensures
    (let ws_s = Spec.ws_pre a block in
     let st_s = shuffle_pre_inner_num_rounds a ws_s i st1 in
     let (ws, st) = shuffle_inner_loop a i (ws1, st1) in
-    st == st_s)
+    st == st_s /\
+   (if i < num_rounds16 a - 1 then
+      ws == Seq.slice ws_s (16 * (i + 1)) (16 * (i + 1) + 16)
+    else
+      ws == Seq.slice ws_s (16 * (num_rounds16 a - 1)) (16 * num_rounds16 a))))
 
 let shuffle_lemma_i_step a block st0 i ws1 st1 =
   let ws_s = Spec.ws_pre a block in
   let st_s = Loops.repeati 16 (shuffle_pre_inner16 a ws_s i) st1 in
   let st = Loops.repeati 16 (shuffle_inner a ws1 i) st1 in
   let ws = if i < num_rounds16 a - 1 then ws_next a ws1 else ws1 in
+  ws_next_inner_lemma a block i ws1;
 
-  let aux (j:nat{j < 16}) (hash:words_state a) :
+  let aux_st (j:nat{j < 16}) (hash:words_state a) :
     Lemma (shuffle_pre_inner16 a ws_s i j hash == shuffle_inner a ws1 i j hash) =
     let k_t = Seq.index (k0 a) (16 * i + j) in
     let lp = shuffle_core_pre a k_t ws_s.[16 * i + j] st in
     let rp = shuffle_core_pre a k_t ws1.[j] hash in
-    assume (ws1.[j] == ws_s.[16 * i + j]);
-    () in
+    assert (ws1.[j] == ws_s.[16 * i + j]) in
 
-  Classical.forall_intro_2 aux;
+  Classical.forall_intro_2 aux_st;
   LSeqLemmas.repeati_extensionality 16 (shuffle_pre_inner16 a ws_s i) (shuffle_inner a ws1 i) st1
+
+
+val ws_pre_init_lemma: a:sha2_alg -> block:k_w a -> Lemma
+  (Seq.slice (Spec.ws_pre a block) 0 16 == block)
+
+let ws_pre_init_lemma a block =
+  reveal_opaque (`%Spec.ws_pre) Spec.ws_pre;
+  let ws0 = Seq.create (Spec.size_k_w a) (to_word a 0) in
+  let ws : Spec.k_w a = Loops.repeati (Spec.size_k_w a) (Spec.ws_pre_inner a block) ws0 in
+  let aux (k:nat{k < 16}) : Lemma (Seq.index ws k == Seq.index block k) =
+    ws_pre_lemma a block (k + 1);
+    ws_pre_lemma_k a block k in
+
+  Classical.forall_intro aux;
+  Seq.lemma_eq_intro (Seq.slice (Spec.ws_pre a block) 0 16) block
 
 
 val shuffle_lemma_i:
@@ -167,7 +527,11 @@ val shuffle_lemma_i:
   (let ws_s = Spec.ws_pre a block in
    let (ws, st) : tuple2 (k_w a) (words_state a) =
      Loops.repeati i (shuffle_inner_loop a) (block, st0) in
-   st == Loops.repeati i (shuffle_pre_inner_num_rounds a ws_s) st0)
+   st == Loops.repeati i (shuffle_pre_inner_num_rounds a ws_s) st0 /\
+   (if i < num_rounds16 a - 1 then
+     ws == Seq.slice ws_s (16 * i) (16 * i + 16)
+    else
+     ws == Seq.slice ws_s (16 * (num_rounds16 a - 1)) (16 * num_rounds16 a)))
 
 let rec shuffle_lemma_i a block st0 i =
   let ws_s = Spec.ws_pre a block in
@@ -177,6 +541,7 @@ let rec shuffle_lemma_i a block st0 i =
   if i = 0 then begin
     Loops.eq_repeati0 i (shuffle_inner_loop a) (block, st0);
     Loops.eq_repeati0 i (shuffle_pre_inner_num_rounds a ws_s) st0;
+    ws_pre_init_lemma a block;
     () end
   else begin
     let (ws1, st1) = Loops.repeati (i - 1) (shuffle_inner_loop a) (block, st0) in
@@ -528,7 +893,7 @@ let update_last_is_repeat_blocks_multi a len last st1 =
     assert (st3 == repeat_blocks_f blocksize blocks1 (update a) nb 1 st2) end
 
 
-#push-options "--z3rlimit 100"
+#push-options "--z3rlimit 150"
 val hash_is_repeat_blocks_multi:
     a:sha2_alg
   -> len:size_nat
